regression tests bpl files updated to better reflect globals names

Dependency/Test/regression/Test0.bpl
@@ -24,6 +24,8 @@ function {:extern} Base(int) : int;
 
 axiom (forall x: int :: { Base(x) } INT_LEQ(Base(x), x));
 
+function {:extern} DT(int) : name;
+
 var {:extern} Mem_T.CHAR: [int]int;
 
 var {:extern} Mem_T.FLOAT: [int]int;
@@ -76,6 +78,11 @@ function {:extern}  INT_SUB(x: int, y: int) : int
   x - y
 }
 
+function {:extern}  INT_MULT(x: int, y: int) : int
+{
+  x * y
+}
+
 function {:extern}  INT_LT(x: int, y: int) : bool
 {
   x < y
@@ -116,19 +123,71 @@ function {:extern}  INT_UGEQ(x: int, y: int) : bool
   x >= y
 }
 
-function {:extern} INT_AND(a: int, b: int) : int;
+function {:extern}  BV32_EQ(x: bv32, y: bv32) : bool
+{
+  x == y
+}
 
-axiom (forall a: int, b: int :: { INT_AND(a, b) } a == b ==> INT_AND(a, b) == a);
+function {:extern}  BV32_NEQ(x: bv32, y: bv32) : bool
+{
+  x != y
+}
 
-axiom (forall a: int, b: int :: { INT_AND(a, b) } POW2(a) && POW2(b) && a != b ==> INT_AND(a, b) == 0);
+function {:extern} {:bvbuiltin "bvadd"} BV32_ADD(x: bv32, y: bv32) : bv32;
 
-axiom (forall a: int, b: int :: { INT_AND(a, b) } a == 0 || b == 0 ==> INT_AND(a, b) == 0);
+function {:extern} {:bvbuiltin "bvsub"} BV32_SUB(x: bv32, y: bv32) : bv32;
 
-function {:extern} INT_OR(a: int, b: int) : int;
+function {:extern} {:bvbuiltin "bvmul"} BV32_MULT(x: bv32, y: bv32) : bv32;
 
-function {:extern} INT_XOR(a: int, b: int) : int;
+function {:extern} {:bvbuiltin "bvudiv"} BV32_DIV(x: bv32, y: bv32) : bv32;
 
-function {:extern} INT_NOT(a: int) : int;
+function {:extern} {:bvbuiltin "bvult"} BV32_ULT(x: bv32, y: bv32) : bool;
+
+function {:extern} {:bvbuiltin "bvslt"} BV32_LT(x: bv32, y: bv32) : bool;
+
+function {:extern} {:bvbuiltin "bvule"} BV32_ULEQ(x: bv32, y: bv32) : bool;
+
+function {:extern} {:bvbuiltin "bvsle"} BV32_LEQ(x: bv32, y: bv32) : bool;
+
+function {:extern} {:bvbuiltin "bvugt"} BV32_UGT(x: bv32, y: bv32) : bool;
+
+function {:extern} {:bvbuiltin "bvsgt"} BV32_GT(x: bv32, y: bv32) : bool;
+
+function {:extern} {:bvbuiltin "bvuge"} BV32_UGEQ(x: bv32, y: bv32) : bool;
+
+function {:extern} {:bvbuiltin "bvsge"} BV32_GEQ(x: bv32, y: bv32) : bool;
+
+function {:extern} MINUS_BOTH_PTR_OR_BOTH_INT(a: int, b: int, size: int) : int;
+
+axiom (forall a: int, b: int, size: int :: { MINUS_BOTH_PTR_OR_BOTH_INT(a, b, size) } INT_LEQ(INT_MULT(size, MINUS_BOTH_PTR_OR_BOTH_INT(a, b, size)), INT_SUB(a, b)) && INT_LT(INT_SUB(a, b), INT_MULT(size, INT_ADD(MINUS_BOTH_PTR_OR_BOTH_INT(a, b, size), 1))));
+
+axiom (forall a: int, b: int, size: int :: { MINUS_BOTH_PTR_OR_BOTH_INT(a, b, size) } MINUS_BOTH_PTR_OR_BOTH_INT(a, b, 1) == INT_SUB(a, b));
+
+function {:extern} MINUS_LEFT_PTR(a: int, a_size: int, b: int) : int;
+
+axiom (forall a: int, a_size: int, b: int :: { MINUS_LEFT_PTR(a, a_size, b) } MINUS_LEFT_PTR(a, a_size, b) == INT_SUB(a, INT_MULT(a_size, b)));
+
+function {:extern} PLUS(a: int, a_size: int, b: int) : int;
+
+axiom (forall a: int, a_size: int, b: int :: { PLUS(a, a_size, b) } PLUS(a, a_size, b) == INT_ADD(a, INT_MULT(a_size, b)));
+
+function {:extern} MULT(a: int, b: int) : int;
+
+axiom (forall a: int, b: int :: { MULT(a, b) } MULT(a, b) == INT_MULT(a, b));
+
+function {:extern} DIV(a: int, b: int) : int;
+
+function {:extern} BINARY_UNKNOWN(a: int, b: int) : int;
+
+axiom (forall a: int, b: int :: { DIV(a, b) } a >= 0 && b > 0 ==> b * DIV(a, b) <= a && a < b * (DIV(a, b) + 1));
+
+axiom (forall a: int, b: int :: { DIV(a, b) } a >= 0 && b < 0 ==> b * DIV(a, b) <= a && a < b * (DIV(a, b) - 1));
+
+axiom (forall a: int, b: int :: { DIV(a, b) } a < 0 && b > 0 ==> b * DIV(a, b) >= a && a > b * (DIV(a, b) - 1));
+
+axiom (forall a: int, b: int :: { DIV(a, b) } a < 0 && b < 0 ==> b * DIV(a, b) >= a && a > b * (DIV(a, b) + 1));
+
+function {:extern} BINARY_BOTH_INT(a: int, b: int) : int;
 
 function {:extern} POW2(a: int) : bool;
 
@@ -184,96 +243,19 @@ axiom POW2(16777216);
 
 axiom POW2(33554432);
 
-function {:extern} INT_MINUS_BOTH_PTR_OR_BOTH_INT(a: int, b: int, size: int) : int;
+function {:extern} BIT_BAND(a: int, b: int) : int;
 
-axiom (forall a: int, b: int, size: int :: { INT_MINUS_BOTH_PTR_OR_BOTH_INT(a, b, size) } size * INT_MINUS_BOTH_PTR_OR_BOTH_INT(a, b, size) <= a - b && a - b < size * (INT_MINUS_BOTH_PTR_OR_BOTH_INT(a, b, size) + 1));
+axiom (forall a: int, b: int :: { BIT_BAND(a, b) } a == b ==> BIT_BAND(a, b) == a);
 
-function {:extern} INT_MINUS_LEFT_PTR(a: int, a_size: int, b: int) : int;
+axiom (forall a: int, b: int :: { BIT_BAND(a, b) } POW2(a) && POW2(b) && a != b ==> BIT_BAND(a, b) == 0);
 
-axiom (forall a: int, a_size: int, b: int :: { INT_MINUS_LEFT_PTR(a, a_size, b) } INT_MINUS_LEFT_PTR(a, a_size, b) == a - a_size * b);
+axiom (forall a: int, b: int :: { BIT_BAND(a, b) } a == 0 || b == 0 ==> BIT_BAND(a, b) == 0);
 
-function {:extern} INT_PLUS(a: int, a_size: int, b: int) : int;
+function {:extern} BIT_BOR(a: int, b: int) : int;
 
-axiom (forall a: int, a_size: int, b: int :: { INT_PLUS(a, a_size, b) } INT_PLUS(a, a_size, b) == a + a_size * b);
+function {:extern} BIT_BXOR(a: int, b: int) : int;
 
-function {:extern} INT_MULT(a: int, b: int) : int;
-
-axiom (forall a: int, b: int :: { INT_MULT(a, b) } INT_MULT(a, b) == a * b);
-
-function {:extern} INT_DIV(a: int, b: int) : int;
-
-axiom (forall a: int, b: int :: { INT_DIV(a, b) } a >= 0 && b > 0 ==> b * INT_DIV(a, b) <= a && a < b * (INT_DIV(a, b) + 1));
-
-axiom (forall a: int, b: int :: { INT_DIV(a, b) } a >= 0 && b < 0 ==> b * INT_DIV(a, b) <= a && a < b * (INT_DIV(a, b) - 1));
-
-axiom (forall a: int, b: int :: { INT_DIV(a, b) } a < 0 && b > 0 ==> b * INT_DIV(a, b) >= a && a > b * (INT_DIV(a, b) - 1));
-
-axiom (forall a: int, b: int :: { INT_DIV(a, b) } a < 0 && b < 0 ==> b * INT_DIV(a, b) >= a && a > b * (INT_DIV(a, b) + 1));
-
-function {:extern} INT_BINARY_BOTH_INT(a: int, b: int) : int;
-
-function {:extern}  BV32_EQ(x: bv32, y: bv32) : bool
-{
-  x == y
-}
-
-function {:extern}  BV32_NEQ(x: bv32, y: bv32) : bool
-{
-  x != y
-}
-
-function {:extern} {:bvbuiltin "bvadd"} BV32_ADD(x: bv32, y: bv32) : bv32;
-
-function {:extern} {:bvbuiltin "bvsub"} BV32_SUB(x: bv32, y: bv32) : bv32;
-
-function {:extern} {:bvbuiltin "bvmul"} BV32_MULT(x: bv32, y: bv32) : bv32;
-
-function {:extern} {:bvbuiltin "bvudiv"} BV32_DIV(x: bv32, y: bv32) : bv32;
-
-function {:extern} {:bvbuiltin "bvult"} BV32_ULT(x: bv32, y: bv32) : bool;
-
-function {:extern} {:bvbuiltin "bvslt"} BV32_LT(x: bv32, y: bv32) : bool;
-
-function {:extern} {:bvbuiltin "bvule"} BV32_ULEQ(x: bv32, y: bv32) : bool;
-
-function {:extern} {:bvbuiltin "bvsle"} BV32_LEQ(x: bv32, y: bv32) : bool;
-
-function {:extern} {:bvbuiltin "bvugt"} BV32_UGT(x: bv32, y: bv32) : bool;
-
-function {:extern} {:bvbuiltin "bvsgt"} BV32_GT(x: bv32, y: bv32) : bool;
-
-function {:extern} {:bvbuiltin "bvuge"} BV32_UGEQ(x: bv32, y: bv32) : bool;
-
-function {:extern} {:bvbuiltin "bvsge"} BV32_GEQ(x: bv32, y: bv32) : bool;
-
-function {:extern} {:bvbuiltin "bvand"} BV32_AND(a: bv32, b: bv32) : bv32;
-
-function {:extern} {:bvbuiltin "bvor"} BV32_OR(a: bv32, b: bv32) : bv32;
-
-function {:extern} {:bvbuiltin "bvxor"} BV32_XOR(a: bv32, b: bv32) : bv32;
-
-function {:extern} {:bvbuiltin "bvnot"} BV32_NOT(a: bv32) : bv32;
-
-function {:extern}  BV32_MINUS_BOTH_PTR_OR_BOTH_INT(a: bv32, b: bv32, size: bv32) : bv32
-{
-  BV32_DIV(BV32_SUB(a, b), size)
-}
-
-function {:extern}  BV32_MINUS_LEFT_PTR(a: bv32, a_size: bv32, b: bv32) : bv32
-{
-  BV32_SUB(a, BV32_MULT(a_size, b))
-}
-
-function {:extern}  BV32_PLUS(a: bv32, a_size: bv32, b: bv32) : bv32
-{
-  BV32_ADD(a, BV32_MULT(a_size, b))
-}
-
-function {:extern} BV32_BINARY_BOTH_INT(a: bv32, b: bv32) : bv32;
-
-function {:extern} bv32ToInt(bv32) : int;
-
-function {:extern} intToBv32(int) : bv32;
+function {:extern} BIT_BNOT(a: int) : int;
 
 function {:extern} choose(a: bool, b: int, c: int) : int;
 
@@ -314,23 +296,21 @@ procedure {:extern} __HAVOC_free(a: int);
 function {:extern} NewAlloc(x: int, y: int) : int;
 
 procedure {:extern} __HAVOC_malloc(obj_size: int) returns (new: int);
-  requires INT_GEQ(obj_size, 0);
+  free requires INT_GEQ(obj_size, 0);
   modifies alloc;
   ensures new == old(alloc);
   ensures INT_GT(alloc, INT_ADD(new, obj_size));
   ensures Base(new) == new;
-  ensures INT_GEQ(new, 0);
 
 
 
 procedure {:extern} __HAVOC_det_malloc(obj_size: int) returns (new: int);
-  requires INT_GEQ(obj_size, 0);
+  free requires INT_GEQ(obj_size, 0);
   modifies alloc;
   ensures new == old(alloc);
   ensures INT_GT(alloc, INT_ADD(new, obj_size));
   ensures Base(new) == new;
   ensures alloc == NewAlloc(old(alloc), obj_size);
-  ensures INT_GEQ(new, 0);
 
 
 
@@ -352,6 +332,10 @@ procedure {:extern} __HAVOC_memset_split_4(A: [int]int, p: int, c: int, n: int) 
 
 
 
+procedure {:extern} nondet_intrinsic() returns (x: int);
+
+
+
 procedure {:extern} nondet_choice() returns (x: int);
 
 
@@ -361,7 +345,6 @@ var {:extern} detChoiceCnt: int;
 function {:extern} DetChoiceFunc(a: int) : int;
 
 procedure {:extern} det_choice() returns (x: int);
-  modifies detChoiceCnt;
   ensures detChoiceCnt == INT_ADD(old(detChoiceCnt), 1);
   ensures x == DetChoiceFunc(old(detChoiceCnt));
 
@@ -378,10 +361,6 @@ procedure {:extern} _xstrcasecmp(a0: int, a1: int) returns (ret: int);
 procedure {:extern} _xstrcmp(a0: int, a1: int) returns (ret: int);
 
 
-
-var {:extern} Res_KERNEL_SOURCE: [int]int;
-
-var {:extern} Res_PROBED: [int]int;
 
 function {:extern} Equal([int]bool, [int]bool) : bool;
 
@@ -417,7 +396,7 @@ axiom (forall n: int, x: int, y: int :: { AtLeast(n, x), Rep(n, x), Rep(n, y) } 
 
 axiom (forall n: int, x: int :: { AtLeast(n, x) } AtLeast(n, x)[x]);
 
-axiom (forall n: int, x: int, z: int :: { INT_PLUS(x, n, z) } Rep(n, x) == Rep(n, INT_PLUS(x, n, z)));
+axiom (forall n: int, x: int, z: int :: { PLUS(x, n, z) } Rep(n, x) == Rep(n, PLUS(x, n, z)));
 
 axiom (forall n: int, x: int :: { Rep(n, x) } (exists k: int :: INT_SUB(Rep(n, x), x) == INT_MULT(n, k)));
 
@@ -425,7 +404,7 @@ function {:extern} Array(int, int, int) : [int]bool;
 
 axiom (forall x: int, n: int, z: int :: { Array(x, n, z) } INT_LEQ(z, 0) ==> Equal(Array(x, n, z), Empty()));
 
-axiom (forall x: int, n: int, z: int :: { Array(x, n, z) } INT_GT(z, 0) ==> Equal(Array(x, n, z), Difference(AtLeast(n, x), AtLeast(n, INT_PLUS(x, n, z)))));
+axiom (forall x: int, n: int, z: int :: { Array(x, n, z) } INT_GT(z, 0) ==> Equal(Array(x, n, z), Difference(AtLeast(n, x), AtLeast(n, PLUS(x, n, z)))));
 
 axiom (forall x: int :: !Empty()[x]);
 
@@ -475,116 +454,92 @@ axiom (forall M: [name][int]int, x: int :: { Unified(M)[x] } Unified(M)[x] == M[
 
 axiom (forall M: [name][int]int, x: int, y: int :: { Unified(M[Field(x) := M[Field(x)][x := y]]) } Unified(M[Field(x) := M[Field(x)][x := y]]) == Unified(M)[x := y]);
 
-const {:extern} unique global1: int;
+var {:extern} global1: int;
 
-axiom INT_GT(global1, 0);
+var {:extern} global2: int;
 
-axiom Base(global1) == global1;
+var {:extern} global3: int;
 
-const {:extern} unique global2: int;
+var {:extern} global4: int;
 
-axiom INT_GT(global2, 0);
-
-axiom Base(global2) == global2;
-
-const {:extern} unique global3: int;
-
-axiom INT_GT(global3, 0);
-
-axiom Base(global3) == global3;
-
-const {:extern} unique global4: int;
-
-axiom INT_GT(global4, 0);
-
-axiom Base(global4) == global4;
-
-const {:extern} unique global5: int;
-
-axiom INT_GT(global5, 0);
-
-axiom Base(global5) == global5;
+var {:extern} global5: int;
 
 const {:extern} unique BOOGIE_FLOAT_CONST_0: int;
 
 function {:extern} value_is(c: int, e: int) : bool;
 
-const {:extern} {:model_const "y"} {:sourceFile "c:\users\t-nisebb\documents\symdiff.src\dependency\test\build\v1\example.c"} {:sourceLine 17} unique __ctobpl_const_2: int;
+const {:extern} {:model_const "global1"} {:sourceFile "c$$users\t-nisebb\documents\symdiff.src\dependency\test\build\regression\test0\test0.c"} {:sourceLine 10} unique __ctobpl_const_1: int;
 
-const {:extern} {:model_const "global1"} {:sourceFile "c:\users\t-nisebb\documents\symdiff.src\dependency\test\build\v1\example.c"} {:sourceLine 10} unique __ctobpl_const_1: int;
+const {:extern} {:model_const "w"} {:sourceFile "c$$users\t-nisebb\documents\symdiff.src\dependency\test\build\regression\test0\test0.c"} {:sourceLine 20} unique __ctobpl_const_3: int;
 
-const {:extern} {:model_const "x"} {:sourceFile "c:\users\t-nisebb\documents\symdiff.src\dependency\test\build\v1\example.c"} {:sourceLine 92} unique __ctobpl_const_8: int;
+const {:extern} {:model_const "y"} {:sourceFile "c$$users\t-nisebb\documents\symdiff.src\dependency\test\build\regression\test0\test0.c"} {:sourceLine 17} unique __ctobpl_const_2: int;
 
-const {:extern} {:model_const "x"} {:sourceFile "c:\users\t-nisebb\documents\symdiff.src\dependency\test\build\v1\example.c"} {:sourceLine 44} unique __ctobpl_const_9: int;
+const {:extern} {:model_const "global2"} {:sourceFile "c$$users\t-nisebb\documents\symdiff.src\dependency\test\build\regression\test0\test0.c"} {:sourceLine 51} unique __ctobpl_const_12: int;
 
-const {:extern} {:model_const "y"} {:sourceFile "c:\users\t-nisebb\documents\symdiff.src\dependency\test\build\v1\example.c"} {:sourceLine 26} unique __ctobpl_const_4: int;
+const {:extern} {:model_const "x"} {:sourceFile "c$$users\t-nisebb\documents\symdiff.src\dependency\test\build\regression\test0\test0.c"} {:sourceLine 52} unique __ctobpl_const_15: int;
 
-const {:extern} {:model_const "w"} {:sourceFile "c:\users\t-nisebb\documents\symdiff.src\dependency\test\build\v1\example.c"} {:sourceLine 29} unique __ctobpl_const_5: int;
+const {:extern} {:model_const "x"} {:sourceFile "c$$users\t-nisebb\documents\symdiff.src\dependency\test\build\regression\test0\test0.c"} {:sourceLine 59} unique __ctobpl_const_18: int;
 
-const {:extern} {:model_const "w"} {:sourceFile "c:\users\t-nisebb\documents\symdiff.src\dependency\test\build\v1\example.c"} {:sourceLine 27} unique __ctobpl_const_6: int;
+const {:extern} {:model_const "x"} {:sourceFile "c$$users\t-nisebb\documents\symdiff.src\dependency\test\build\regression\test0\test0.c"} {:sourceLine 59} unique __ctobpl_const_19: int;
 
-const {:extern} {:model_const "result.TestCallDominationDependancyCalleeConst"} {:sourceFile "c:\users\t-nisebb\documents\symdiff.src\dependency\test\build\v1\example.c"} {:sourceLine 27} unique __ctobpl_const_7: int;
+const {:extern} {:model_const "x"} {:sourceFile "c$$users\t-nisebb\documents\symdiff.src\dependency\test\build\regression\test0\test0.c"} {:sourceLine 35} unique __ctobpl_const_30: int;
 
-const {:extern} {:model_const "w"} {:sourceFile "c:\users\t-nisebb\documents\symdiff.src\dependency\test\build\v1\example.c"} {:sourceLine 20} unique __ctobpl_const_3: int;
+const {:extern} {:model_const "x"} {:sourceFile "c$$users\t-nisebb\documents\symdiff.src\dependency\test\build\regression\test0\test0.c"} {:sourceLine 44} unique __ctobpl_const_10: int;
 
-const {:extern} {:model_const "x"} {:sourceFile "c:\users\t-nisebb\documents\symdiff.src\dependency\test\build\v1\example.c"} {:sourceLine 44} unique __ctobpl_const_10: int;
+const {:extern} {:model_const "result.TestCallDominationDependancyCalleeConst"} {:sourceFile "c$$users\t-nisebb\documents\symdiff.src\dependency\test\build\regression\test0\test0.c"} {:sourceLine 27} unique __ctobpl_const_6: int;
 
-const {:extern} {:model_const "result.TestEmptyRecursion"} {:sourceFile "c:\users\t-nisebb\documents\symdiff.src\dependency\test\build\v1\example.c"} {:sourceLine 44} unique __ctobpl_const_11: int;
+const {:extern} {:model_const "x"} {:sourceFile "c$$users\t-nisebb\documents\symdiff.src\dependency\test\build\regression\test0\test0.c"} {:sourceLine 52} unique __ctobpl_const_14: int;
 
-const {:extern} {:model_const "result.TestGlobalRecursion"} {:sourceFile "c:\users\t-nisebb\documents\symdiff.src\dependency\test\build\v1\example.c"} {:sourceLine 52} unique __ctobpl_const_16: int;
+const {:extern} {:model_const "result.TestGlobalRecursion"} {:sourceFile "c$$users\t-nisebb\documents\symdiff.src\dependency\test\build\regression\test0\test0.c"} {:sourceLine 52} unique __ctobpl_const_16: int;
 
-const {:extern} {:model_const "y"} {:sourceFile "c:\users\t-nisebb\documents\symdiff.src\dependency\test\build\v1\example.c"} {:sourceLine 79} unique __ctobpl_const_26: int;
+const {:extern} {:model_const "global4"} {:sourceFile "c$$users\t-nisebb\documents\symdiff.src\dependency\test\build\regression\test0\test0.c"} {:sourceLine 72} unique __ctobpl_const_22: int;
 
-const {:extern} {:model_const "x"} {:sourceFile "c:\users\t-nisebb\documents\symdiff.src\dependency\test\build\v1\example.c"} {:sourceLine 59} unique __ctobpl_const_19: int;
+const {:extern} {:model_const "x"} {:sourceFile "c$$users\t-nisebb\documents\symdiff.src\dependency\test\build\regression\test0\test0.c"} {:sourceLine 73} unique __ctobpl_const_23: int;
 
-const {:extern} {:model_const "global4"} {:sourceFile "c:\users\t-nisebb\documents\symdiff.src\dependency\test\build\v1\example.c"} {:sourceLine 72} unique __ctobpl_const_22: int;
+const {:extern} {:model_const "global3"} {:sourceFile "c$$users\t-nisebb\documents\symdiff.src\dependency\test\build\regression\test0\test0.c"} {:sourceLine 80} unique __ctobpl_const_27: int;
 
-const {:extern} {:model_const "global5"} {:sourceFile "c:\users\t-nisebb\documents\symdiff.src\dependency\test\build\v1\example.c"} {:sourceLine 78} unique __ctobpl_const_24: int;
+const {:extern} {:model_const "x"} {:sourceFile "c$$users\t-nisebb\documents\symdiff.src\dependency\test\build\regression\test0\test0.c"} {:sourceLine 34} unique __ctobpl_const_28: int;
 
-const {:extern} {:model_const "x"} {:sourceFile "c:\users\t-nisebb\documents\symdiff.src\dependency\test\build\v1\example.c"} {:sourceLine 51} unique __ctobpl_const_13: int;
+const {:extern} {:model_const "y"} {:sourceFile "c$$users\t-nisebb\documents\symdiff.src\dependency\test\build\regression\test0\test0.c"} {:sourceLine 26} unique __ctobpl_const_4: int;
 
-const {:extern} {:model_const "global3"} {:sourceFile "c:\users\t-nisebb\documents\symdiff.src\dependency\test\build\v1\example.c"} {:sourceLine 80} unique __ctobpl_const_27: int;
+const {:extern} {:model_const "w"} {:sourceFile "c$$users\t-nisebb\documents\symdiff.src\dependency\test\build\regression\test0\test0.c"} {:sourceLine 37} unique __ctobpl_const_33: int;
 
-const {:extern} {:model_const "w"} {:sourceFile "c:\users\t-nisebb\documents\symdiff.src\dependency\test\build\v1\example.c"} {:sourceLine 39} unique __ctobpl_const_31: int;
+const {:extern} {:model_const "result.TestRecursion"} {:sourceFile "c$$users\t-nisebb\documents\symdiff.src\dependency\test\build\regression\test0\test0.c"} {:sourceLine 59} unique __ctobpl_const_20: int;
 
-const {:extern} {:model_const "x"} {:sourceFile "c:\users\t-nisebb\documents\symdiff.src\dependency\test\build\v1\example.c"} {:sourceLine 52} unique __ctobpl_const_14: int;
+const {:extern} {:model_const "z"} {:sourceFile "c$$users\t-nisebb\documents\symdiff.src\dependency\test\build\regression\test0\test0.c"} {:sourceLine 71} unique __ctobpl_const_21: int;
 
-const {:extern} {:model_const "x"} {:sourceFile "c:\users\t-nisebb\documents\symdiff.src\dependency\test\build\v1\example.c"} {:sourceLine 36} unique __ctobpl_const_32: int;
+const {:extern} {:model_const "y"} {:sourceFile "c$$users\t-nisebb\documents\symdiff.src\dependency\test\build\regression\test0\test0.c"} {:sourceLine 79} unique __ctobpl_const_26: int;
 
-const {:extern} {:model_const "x"} {:sourceFile "c:\users\t-nisebb\documents\symdiff.src\dependency\test\build\v1\example.c"} {:sourceLine 34} unique __ctobpl_const_28: int;
+const {:extern} {:model_const "x"} {:sourceFile "c$$users\t-nisebb\documents\symdiff.src\dependency\test\build\regression\test0\test0.c"} {:sourceLine 36} unique __ctobpl_const_31: int;
 
-const {:extern} {:model_const "z"} {:sourceFile "c:\users\t-nisebb\documents\symdiff.src\dependency\test\build\v1\example.c"} {:sourceLine 36} unique __ctobpl_const_33: int;
+const {:extern} {:model_const "x"} {:sourceFile "c$$users\t-nisebb\documents\symdiff.src\dependency\test\build\regression\test0\test0.c"} {:sourceLine 44} unique __ctobpl_const_9: int;
 
-const {:extern} {:model_const "w"} {:sourceFile "c:\users\t-nisebb\documents\symdiff.src\dependency\test\build\v1\example.c"} {:sourceLine 74} unique __ctobpl_const_25: int;
+const {:extern} {:model_const "x"} {:sourceFile "c$$users\t-nisebb\documents\symdiff.src\dependency\test\build\regression\test0\test0.c"} {:sourceLine 57} unique __ctobpl_const_17: int;
 
-const {:extern} {:model_const "x"} {:sourceFile "c:\users\t-nisebb\documents\symdiff.src\dependency\test\build\v1\example.c"} {:sourceLine 73} unique __ctobpl_const_23: int;
+const {:extern} {:model_const "y"} {:sourceFile "c$$users\t-nisebb\documents\symdiff.src\dependency\test\build\regression\test0\test0.c"} {:sourceLine 34} unique __ctobpl_const_29: int;
 
-const {:extern} {:model_const "y"} {:sourceFile "c:\users\t-nisebb\documents\symdiff.src\dependency\test\build\v1\example.c"} {:sourceLine 34} unique __ctobpl_const_29: int;
+const {:extern} {:model_const "w"} {:sourceFile "c$$users\t-nisebb\documents\symdiff.src\dependency\test\build\regression\test0\test0.c"} {:sourceLine 74} unique __ctobpl_const_25: int;
 
-const {:extern} {:model_const "x"} {:sourceFile "c:\users\t-nisebb\documents\symdiff.src\dependency\test\build\v1\example.c"} {:sourceLine 59} unique __ctobpl_const_18: int;
+const {:extern} {:model_const "w"} {:sourceFile "c$$users\t-nisebb\documents\symdiff.src\dependency\test\build\regression\test0\test0.c"} {:sourceLine 29} unique __ctobpl_const_7: int;
 
-const {:extern} {:model_const "global2"} {:sourceFile "c:\users\t-nisebb\documents\symdiff.src\dependency\test\build\v1\example.c"} {:sourceLine 51} unique __ctobpl_const_12: int;
+const {:extern} {:model_const "z"} {:sourceFile "c$$users\t-nisebb\documents\symdiff.src\dependency\test\build\regression\test0\test0.c"} {:sourceLine 36} unique __ctobpl_const_32: int;
 
-const {:extern} {:model_const "x"} {:sourceFile "c:\users\t-nisebb\documents\symdiff.src\dependency\test\build\v1\example.c"} {:sourceLine 52} unique __ctobpl_const_15: int;
+const {:extern} {:model_const "x"} {:sourceFile "c$$users\t-nisebb\documents\symdiff.src\dependency\test\build\regression\test0\test0.c"} {:sourceLine 92} unique __ctobpl_const_8: int;
 
-const {:extern} {:model_const "z"} {:sourceFile "c:\users\t-nisebb\documents\symdiff.src\dependency\test\build\v1\example.c"} {:sourceLine 71} unique __ctobpl_const_21: int;
+const {:extern} {:model_const "global5"} {:sourceFile "c$$users\t-nisebb\documents\symdiff.src\dependency\test\build\regression\test0\test0.c"} {:sourceLine 78} unique __ctobpl_const_24: int;
 
-const {:extern} {:model_const "x"} {:sourceFile "c:\users\t-nisebb\documents\symdiff.src\dependency\test\build\v1\example.c"} {:sourceLine 57} unique __ctobpl_const_17: int;
+const {:extern} {:model_const "x"} {:sourceFile "c$$users\t-nisebb\documents\symdiff.src\dependency\test\build\regression\test0\test0.c"} {:sourceLine 51} unique __ctobpl_const_13: int;
 
-const {:extern} {:model_const "result.TestRecursion"} {:sourceFile "c:\users\t-nisebb\documents\symdiff.src\dependency\test\build\v1\example.c"} {:sourceLine 59} unique __ctobpl_const_20: int;
+const {:extern} {:model_const "result.TestEmptyRecursion"} {:sourceFile "c$$users\t-nisebb\documents\symdiff.src\dependency\test\build\regression\test0\test0.c"} {:sourceLine 44} unique __ctobpl_const_11: int;
 
-const {:extern} {:model_const "x"} {:sourceFile "c:\users\t-nisebb\documents\symdiff.src\dependency\test\build\v1\example.c"} {:sourceLine 35} unique __ctobpl_const_30: int;
+const {:extern} {:model_const "w"} {:sourceFile "c$$users\t-nisebb\documents\symdiff.src\dependency\test\build\regression\test0\test0.c"} {:sourceLine 27} unique __ctobpl_const_5: int;
 
-const {:extern} {:model_const "w"} {:sourceFile "c:\users\t-nisebb\documents\symdiff.src\dependency\test\build\v1\example.c"} {:sourceLine 37} unique __ctobpl_const_34: int;
+const {:extern} {:model_const "w"} {:sourceFile "c$$users\t-nisebb\documents\symdiff.src\dependency\test\build\regression\test0\test0.c"} {:sourceLine 39} unique __ctobpl_const_34: int;
 
 procedure {:extern} TestCallDominationDependancyCalleeConst() returns (result.TestCallDominationDependancyCalleeConst$1: int);
   free requires INT_LT(0, alloc);
-  modifies alloc, detChoiceCnt, Res_KERNEL_SOURCE, Res_PROBED, Mem_T.CHAR, Mem_T.FLOAT, Mem_T.INT4;
+  modifies alloc, detChoiceCnt, Mem_T.CHAR, Mem_T.FLOAT, Mem_T.INT4, global1, global2, global3, global4, global5;
   free ensures INT_LEQ(old(alloc), alloc);
-  ensures Subset(Empty(), Empty()) && (forall _r: int :: { Res_KERNEL_SOURCE[_r] } old(Res_KERNEL_SOURCE)[_r] == Res_KERNEL_SOURCE[_r]);
-  free ensures old(Res_KERNEL_SOURCE) == Res_KERNEL_SOURCE;
-  ensures Subset(Empty(), Empty()) && (forall _r: int :: { Res_PROBED[_r] } old(Res_PROBED)[_r] == Res_PROBED[_r]);
-  free ensures old(Res_PROBED) == Res_PROBED;
   free ensures Mem_T.CHAR == old(Mem_T.CHAR);
   free ensures Mem_T.FLOAT == old(Mem_T.FLOAT);
   free ensures Mem_T.INT4 == old(Mem_T.INT4);
@@ -615,7 +570,6 @@ implementation {:extern} TestCallDominationDependancyCalleeConst() returns (resu
   var {:extern} tempBoogie17: int;
   var {:extern} tempBoogie18: int;
   var {:extern} tempBoogie19: int;
-  var {:extern} __havoc_dummy_return: int;
 
   anon0#2:
     havoc_stringTemp := 0;
@@ -626,12 +580,12 @@ implementation {:extern} TestCallDominationDependancyCalleeConst() returns (resu
     goto label_3#2;
 
   label_3#2:
-    assert {:sourcefile "c:\users\t-nisebb\documents\symdiff.src\dependency\test\build\v1\example.c"} {:sourceline 3} true;
+    assert {:sourcefile "c$$users\t-nisebb\documents\symdiff.src\dependency\test\build\regression\test0\test0.c"} {:sourceline 3} true;
     result.TestCallDominationDependancyCalleeConst$1 := 0;
     goto label_1#2;
 
   label_1#2:
-    assert {:sourcefile "c:\users\t-nisebb\documents\symdiff.src\dependency\test\build\v1\example.c"} {:sourceline 4} true;
+    assert {:sourcefile "c$$users\t-nisebb\documents\symdiff.src\dependency\test\build\regression\test0\test0.c"} {:sourceline 4} true;
     return;
 }
 
@@ -639,12 +593,8 @@ implementation {:extern} TestCallDominationDependancyCalleeConst() returns (resu
 
 procedure {:extern} TestCallDominationDependancyCalleeGlobals();
   free requires INT_LT(0, alloc);
-  modifies alloc, detChoiceCnt, Res_KERNEL_SOURCE, Res_PROBED, Mem_T.CHAR, Mem_T.FLOAT, Mem_T.INT4;
+  modifies alloc, detChoiceCnt, Mem_T.CHAR, Mem_T.FLOAT, Mem_T.INT4, global1, global2, global3, global4, global5;
   free ensures INT_LEQ(old(alloc), alloc);
-  ensures Subset(Empty(), Empty()) && (forall _r: int :: { Res_KERNEL_SOURCE[_r] } old(Res_KERNEL_SOURCE)[_r] == Res_KERNEL_SOURCE[_r]);
-  free ensures old(Res_KERNEL_SOURCE) == Res_KERNEL_SOURCE;
-  ensures Subset(Empty(), Empty()) && (forall _r: int :: { Res_PROBED[_r] } old(Res_PROBED)[_r] == Res_PROBED[_r]);
-  free ensures old(Res_PROBED) == Res_PROBED;
   free ensures Mem_T.CHAR == old(Mem_T.CHAR);
   free ensures Mem_T.FLOAT == old(Mem_T.FLOAT);
   free ensures Mem_T.INT4 == old(Mem_T.INT4);
@@ -675,7 +625,6 @@ implementation {:extern} TestCallDominationDependancyCalleeGlobals()
   var {:extern} tempBoogie17: int;
   var {:extern} tempBoogie18: int;
   var {:extern} tempBoogie19: int;
-  var {:extern} __havoc_dummy_return: int;
 
   anon0#2:
     havoc_stringTemp := 0;
@@ -685,34 +634,29 @@ implementation {:extern} TestCallDominationDependancyCalleeGlobals()
     goto label_3#2;
 
   label_3#2:
-    assert {:sourcefile "c:\users\t-nisebb\documents\symdiff.src\dependency\test\build\v1\example.c"} {:sourceline 10} true;
-    assume value_is(__ctobpl_const_1, Mem_T.INT4[global1]);
-    tempBoogie0 := INT_PLUS(Mem_T.INT4[global1], 1, 1);
-    Mem_T.INT4 := Mem_T.INT4[global1 := tempBoogie0];
+    assert {:sourcefile "c$$users\t-nisebb\documents\symdiff.src\dependency\test\build\regression\test0\test0.c"} {:sourceline 10} true;
+    assume value_is(__ctobpl_const_1, global1);
+    global1 := PLUS(global1, 1, 1);
     goto label_1#2;
 
   label_1#2:
-    assert {:sourcefile "c:\users\t-nisebb\documents\symdiff.src\dependency\test\build\v1\example.c"} {:sourceline 11} true;
+    assert {:sourcefile "c$$users\t-nisebb\documents\symdiff.src\dependency\test\build\regression\test0\test0.c"} {:sourceline 11} true;
     return;
 }
 
 
 
-procedure {:extern} TestCallDominationDependancyGlobals(y_.1: int, z_.1: int) returns (result.TestCallDominationDependancyGlobals$1: int);
+procedure {:extern} TestCallDominationDependancyGlobals(y.__1: int, z.__1: int) returns (result.TestCallDominationDependancyGlobals$1: int);
   free requires INT_LT(0, alloc);
-  modifies alloc, detChoiceCnt, Res_KERNEL_SOURCE, Res_PROBED, Mem_T.CHAR, Mem_T.FLOAT, Mem_T.INT4;
+  modifies alloc, detChoiceCnt, Mem_T.CHAR, Mem_T.FLOAT, Mem_T.INT4, global1, global2, global3, global4, global5;
   free ensures INT_LEQ(old(alloc), alloc);
-  ensures Subset(Empty(), Empty()) && (forall _r: int :: { Res_KERNEL_SOURCE[_r] } old(Res_KERNEL_SOURCE)[_r] == Res_KERNEL_SOURCE[_r]);
-  free ensures old(Res_KERNEL_SOURCE) == Res_KERNEL_SOURCE;
-  ensures Subset(Empty(), Empty()) && (forall _r: int :: { Res_PROBED[_r] } old(Res_PROBED)[_r] == Res_PROBED[_r]);
-  free ensures old(Res_PROBED) == Res_PROBED;
   free ensures Mem_T.CHAR == old(Mem_T.CHAR);
   free ensures Mem_T.FLOAT == old(Mem_T.FLOAT);
   free ensures Mem_T.INT4 == old(Mem_T.INT4);
 
 
 
-implementation {:extern} TestCallDominationDependancyGlobals(y_.1: int, z_.1: int) returns (result.TestCallDominationDependancyGlobals$1: int)
+implementation {:extern} TestCallDominationDependancyGlobals(y.__1: int, z.__1: int) returns (result.TestCallDominationDependancyGlobals$1: int)
 {
   var {:extern} havoc_stringTemp: int;
   var {:extern} condVal: int;
@@ -739,7 +683,6 @@ implementation {:extern} TestCallDominationDependancyGlobals(y_.1: int, z_.1: in
   var {:extern} tempBoogie17: int;
   var {:extern} tempBoogie18: int;
   var {:extern} tempBoogie19: int;
-  var {:extern} __havoc_dummy_return: int;
 
   anon0#2:
     havoc_stringTemp := 0;
@@ -750,16 +693,16 @@ implementation {:extern} TestCallDominationDependancyGlobals(y_.1: int, z_.1: in
     w := 0;
     y := 0;
     z := 0;
-    y := y_.1;
-    z := z_.1;
+    y := y.__1;
+    z := z.__1;
     goto label_3#2;
 
   label_3#2:
-    assert {:sourcefile "c:\users\t-nisebb\documents\symdiff.src\dependency\test\build\v1\example.c"} {:sourceline 16} true;
+    assert {:sourcefile "c$$users\t-nisebb\documents\symdiff.src\dependency\test\build\regression\test0\test0.c"} {:sourceline 16} true;
     goto label_4#2;
 
   label_4#2:
-    assert {:sourcefile "c:\users\t-nisebb\documents\symdiff.src\dependency\test\build\v1\example.c"} {:sourceline 17} true;
+    assert {:sourcefile "c$$users\t-nisebb\documents\symdiff.src\dependency\test\build\regression\test0\test0.c"} {:sourceline 17} true;
     goto label_4_true#2, label_4_false#2;
 
   label_4_false#2:
@@ -773,38 +716,34 @@ implementation {:extern} TestCallDominationDependancyGlobals(y_.1: int, z_.1: in
     goto label_6#2;
 
   label_6#2:
-    assert {:sourcefile "c:\users\t-nisebb\documents\symdiff.src\dependency\test\build\v1\example.c"} {:sourceline 18} true;
+    assert {:sourcefile "c$$users\t-nisebb\documents\symdiff.src\dependency\test\build\regression\test0\test0.c"} {:sourceline 18} true;
     call TestCallDominationDependancyCalleeGlobals();
     goto label_5#2;
 
   label_5#2:
-    assert {:sourcefile "c:\users\t-nisebb\documents\symdiff.src\dependency\test\build\v1\example.c"} {:sourceline 20} true;
+    assert {:sourcefile "c$$users\t-nisebb\documents\symdiff.src\dependency\test\build\regression\test0\test0.c"} {:sourceline 20} true;
     result.TestCallDominationDependancyGlobals$1 := w;
     assume value_is(__ctobpl_const_3, w);
     goto label_1#2;
 
   label_1#2:
-    assert {:sourcefile "c:\users\t-nisebb\documents\symdiff.src\dependency\test\build\v1\example.c"} {:sourceline 21} true;
+    assert {:sourcefile "c$$users\t-nisebb\documents\symdiff.src\dependency\test\build\regression\test0\test0.c"} {:sourceline 21} true;
     return;
 }
 
 
 
-procedure {:extern} TestCallDominationDependancyReturns(y_.1: int, z_.1: int) returns (result.TestCallDominationDependancyReturns$1: int);
+procedure {:extern} TestCallDominationDependancyReturns(y.__1: int, z.__1: int) returns (result.TestCallDominationDependancyReturns$1: int);
   free requires INT_LT(0, alloc);
-  modifies alloc, detChoiceCnt, Res_KERNEL_SOURCE, Res_PROBED, Mem_T.CHAR, Mem_T.FLOAT, Mem_T.INT4;
+  modifies alloc, detChoiceCnt, Mem_T.CHAR, Mem_T.FLOAT, Mem_T.INT4, global1, global2, global3, global4, global5;
   free ensures INT_LEQ(old(alloc), alloc);
-  ensures Subset(Empty(), Empty()) && (forall _r: int :: { Res_KERNEL_SOURCE[_r] } old(Res_KERNEL_SOURCE)[_r] == Res_KERNEL_SOURCE[_r]);
-  free ensures old(Res_KERNEL_SOURCE) == Res_KERNEL_SOURCE;
-  ensures Subset(Empty(), Empty()) && (forall _r: int :: { Res_PROBED[_r] } old(Res_PROBED)[_r] == Res_PROBED[_r]);
-  free ensures old(Res_PROBED) == Res_PROBED;
   free ensures Mem_T.CHAR == old(Mem_T.CHAR);
   free ensures Mem_T.FLOAT == old(Mem_T.FLOAT);
   free ensures Mem_T.INT4 == old(Mem_T.INT4);
 
 
 
-implementation {:extern} TestCallDominationDependancyReturns(y_.1: int, z_.1: int) returns (result.TestCallDominationDependancyReturns$1: int)
+implementation {:extern} TestCallDominationDependancyReturns(y.__1: int, z.__1: int) returns (result.TestCallDominationDependancyReturns$1: int)
 {
   var {:extern} havoc_stringTemp: int;
   var {:extern} condVal: int;
@@ -832,7 +771,6 @@ implementation {:extern} TestCallDominationDependancyReturns(y_.1: int, z_.1: in
   var {:extern} tempBoogie17: int;
   var {:extern} tempBoogie18: int;
   var {:extern} tempBoogie19: int;
-  var {:extern} __havoc_dummy_return: int;
 
   anon0#2:
     havoc_stringTemp := 0;
@@ -844,16 +782,16 @@ implementation {:extern} TestCallDominationDependancyReturns(y_.1: int, z_.1: in
     w := 0;
     y := 0;
     z := 0;
-    y := y_.1;
-    z := z_.1;
+    y := y.__1;
+    z := z.__1;
     goto label_3#2;
 
   label_3#2:
-    assert {:sourcefile "c:\users\t-nisebb\documents\symdiff.src\dependency\test\build\v1\example.c"} {:sourceline 25} true;
+    assert {:sourcefile "c$$users\t-nisebb\documents\symdiff.src\dependency\test\build\regression\test0\test0.c"} {:sourceline 25} true;
     goto label_4#2;
 
   label_4#2:
-    assert {:sourcefile "c:\users\t-nisebb\documents\symdiff.src\dependency\test\build\v1\example.c"} {:sourceline 26} true;
+    assert {:sourcefile "c$$users\t-nisebb\documents\symdiff.src\dependency\test\build\regression\test0\test0.c"} {:sourceline 26} true;
     goto label_4_true#2, label_4_false#2;
 
   label_4_false#2:
@@ -867,45 +805,41 @@ implementation {:extern} TestCallDominationDependancyReturns(y_.1: int, z_.1: in
     goto label_6#2;
 
   label_6#2:
-    assert {:sourcefile "c:\users\t-nisebb\documents\symdiff.src\dependency\test\build\v1\example.c"} {:sourceline 27} true;
+    assert {:sourcefile "c$$users\t-nisebb\documents\symdiff.src\dependency\test\build\regression\test0\test0.c"} {:sourceline 27} true;
     call result.TestCallDominationDependancyCalleeConst$2 := TestCallDominationDependancyCalleeConst();
     goto label_9#2;
 
   label_9#2:
-    assert {:sourcefile "c:\users\t-nisebb\documents\symdiff.src\dependency\test\build\v1\example.c"} {:sourceline 27} true;
+    assert {:sourcefile "c$$users\t-nisebb\documents\symdiff.src\dependency\test\build\regression\test0\test0.c"} {:sourceline 27} true;
     w := result.TestCallDominationDependancyCalleeConst$2;
-    assume value_is(__ctobpl_const_6, w);
-    assume value_is(__ctobpl_const_7, result.TestCallDominationDependancyCalleeConst$2);
+    assume value_is(__ctobpl_const_5, w);
+    assume value_is(__ctobpl_const_6, result.TestCallDominationDependancyCalleeConst$2);
     goto label_5#2;
 
   label_5#2:
-    assert {:sourcefile "c:\users\t-nisebb\documents\symdiff.src\dependency\test\build\v1\example.c"} {:sourceline 29} true;
+    assert {:sourcefile "c$$users\t-nisebb\documents\symdiff.src\dependency\test\build\regression\test0\test0.c"} {:sourceline 29} true;
     result.TestCallDominationDependancyReturns$1 := w;
-    assume value_is(__ctobpl_const_5, w);
+    assume value_is(__ctobpl_const_7, w);
     goto label_1#2;
 
   label_1#2:
-    assert {:sourcefile "c:\users\t-nisebb\documents\symdiff.src\dependency\test\build\v1\example.c"} {:sourceline 30} true;
+    assert {:sourcefile "c$$users\t-nisebb\documents\symdiff.src\dependency\test\build\regression\test0\test0.c"} {:sourceline 30} true;
     return;
 }
 
 
 
-procedure {:extern} TestCondExit(x_.1: int) returns (result.TestCondExit$1: int);
+procedure {:extern} TestCondExit(x.__1: int) returns (result.TestCondExit$1: int);
   free requires INT_LT(0, alloc);
-  modifies alloc, detChoiceCnt, Res_KERNEL_SOURCE, Res_PROBED, Mem_T.CHAR, Mem_T.FLOAT, Mem_T.INT4;
+  modifies alloc, detChoiceCnt, Mem_T.CHAR, Mem_T.FLOAT, Mem_T.INT4, global1, global2, global3, global4, global5;
   free ensures INT_LEQ(old(alloc), alloc);
-  ensures Subset(Empty(), Empty()) && (forall _r: int :: { Res_KERNEL_SOURCE[_r] } old(Res_KERNEL_SOURCE)[_r] == Res_KERNEL_SOURCE[_r]);
-  free ensures old(Res_KERNEL_SOURCE) == Res_KERNEL_SOURCE;
-  ensures Subset(Empty(), Empty()) && (forall _r: int :: { Res_PROBED[_r] } old(Res_PROBED)[_r] == Res_PROBED[_r]);
-  free ensures old(Res_PROBED) == Res_PROBED;
   free ensures Mem_T.CHAR == old(Mem_T.CHAR);
   free ensures Mem_T.FLOAT == old(Mem_T.FLOAT);
   free ensures Mem_T.INT4 == old(Mem_T.INT4);
 
 
 
-implementation {:extern} TestCondExit(x_.1: int) returns (result.TestCondExit$1: int)
+implementation {:extern} TestCondExit(x.__1: int) returns (result.TestCondExit$1: int)
 {
   var {:extern} havoc_stringTemp: int;
   var {:extern} condVal: int;
@@ -931,7 +865,6 @@ implementation {:extern} TestCondExit(x_.1: int) returns (result.TestCondExit$1:
   var {:extern} tempBoogie17: int;
   var {:extern} tempBoogie18: int;
   var {:extern} tempBoogie19: int;
-  var {:extern} __havoc_dummy_return: int;
 
   anon0#2:
     havoc_stringTemp := 0;
@@ -941,11 +874,11 @@ implementation {:extern} TestCondExit(x_.1: int) returns (result.TestCondExit$1:
     result.TestCondExit$1 := 0;
     result.exit$2 := 0;
     x := 0;
-    x := x_.1;
+    x := x.__1;
     goto label_3#2;
 
   label_3#2:
-    assert {:sourcefile "c:\users\t-nisebb\documents\symdiff.src\dependency\test\build\v1\example.c"} {:sourceline 92} true;
+    assert {:sourcefile "c$$users\t-nisebb\documents\symdiff.src\dependency\test\build\regression\test0\test0.c"} {:sourceline 92} true;
     goto label_3_true#2, label_3_false#2;
 
   label_3_false#2:
@@ -954,7 +887,7 @@ implementation {:extern} TestCondExit(x_.1: int) returns (result.TestCondExit$1:
     goto label_4#2;
 
   label_4#2:
-    assert {:sourcefile "c:\users\t-nisebb\documents\symdiff.src\dependency\test\build\v1\example.c"} {:sourceline 94} true;
+    assert {:sourcefile "c$$users\t-nisebb\documents\symdiff.src\dependency\test\build\regression\test0\test0.c"} {:sourceline 94} true;
     call result.exit$2 := det_choice();
     assume false;
     return;
@@ -965,32 +898,28 @@ implementation {:extern} TestCondExit(x_.1: int) returns (result.TestCondExit$1:
     goto label_7#2;
 
   label_7#2:
-    assert {:sourcefile "c:\users\t-nisebb\documents\symdiff.src\dependency\test\build\v1\example.c"} {:sourceline 93} true;
+    assert {:sourcefile "c$$users\t-nisebb\documents\symdiff.src\dependency\test\build\regression\test0\test0.c"} {:sourceline 93} true;
     result.TestCondExit$1 := 0;
     goto label_1#2;
 
   label_1#2:
-    assert {:sourcefile "c:\users\t-nisebb\documents\symdiff.src\dependency\test\build\v1\example.c"} {:sourceline 96} true;
+    assert {:sourcefile "c$$users\t-nisebb\documents\symdiff.src\dependency\test\build\regression\test0\test0.c"} {:sourceline 96} true;
     return;
 }
 
 
 
-procedure {:extern} TestEmptyRecursion(x_.1: int) returns (result.TestEmptyRecursion$1: int);
+procedure {:extern} TestEmptyRecursion(x.__1: int) returns (result.TestEmptyRecursion$1: int);
   free requires INT_LT(0, alloc);
-  modifies alloc, detChoiceCnt, Res_KERNEL_SOURCE, Res_PROBED, Mem_T.CHAR, Mem_T.FLOAT, Mem_T.INT4;
+  modifies alloc, detChoiceCnt, Mem_T.CHAR, Mem_T.FLOAT, Mem_T.INT4, global1, global2, global3, global4, global5;
   free ensures INT_LEQ(old(alloc), alloc);
-  ensures Subset(Empty(), Empty()) && (forall _r: int :: { Res_KERNEL_SOURCE[_r] } old(Res_KERNEL_SOURCE)[_r] == Res_KERNEL_SOURCE[_r]);
-  free ensures old(Res_KERNEL_SOURCE) == Res_KERNEL_SOURCE;
-  ensures Subset(Empty(), Empty()) && (forall _r: int :: { Res_PROBED[_r] } old(Res_PROBED)[_r] == Res_PROBED[_r]);
-  free ensures old(Res_PROBED) == Res_PROBED;
   free ensures Mem_T.CHAR == old(Mem_T.CHAR);
   free ensures Mem_T.FLOAT == old(Mem_T.FLOAT);
   free ensures Mem_T.INT4 == old(Mem_T.INT4);
 
 
 
-implementation {:extern} TestEmptyRecursion(x_.1: int) returns (result.TestEmptyRecursion$1: int)
+implementation {:extern} TestEmptyRecursion(x.__1: int) returns (result.TestEmptyRecursion$1: int)
 {
   var {:extern} havoc_stringTemp: int;
   var {:extern} condVal: int;
@@ -1016,7 +945,6 @@ implementation {:extern} TestEmptyRecursion(x_.1: int) returns (result.TestEmpty
   var {:extern} tempBoogie17: int;
   var {:extern} tempBoogie18: int;
   var {:extern} tempBoogie19: int;
-  var {:extern} __havoc_dummy_return: int;
 
   anon0#2:
     havoc_stringTemp := 0;
@@ -1026,44 +954,40 @@ implementation {:extern} TestEmptyRecursion(x_.1: int) returns (result.TestEmpty
     result.TestEmptyRecursion$1 := 0;
     result.TestEmptyRecursion$2 := 0;
     x := 0;
-    x := x_.1;
+    x := x.__1;
     goto label_3#2;
 
   label_3#2:
-    assert {:sourcefile "c:\users\t-nisebb\documents\symdiff.src\dependency\test\build\v1\example.c"} {:sourceline 44} true;
+    assert {:sourcefile "c$$users\t-nisebb\documents\symdiff.src\dependency\test\build\regression\test0\test0.c"} {:sourceline 44} true;
     call result.TestEmptyRecursion$2 := TestEmptyRecursion(x);
     assume value_is(__ctobpl_const_9, x);
     assume value_is(__ctobpl_const_10, x);
     goto label_6#2;
 
   label_6#2:
-    assert {:sourcefile "c:\users\t-nisebb\documents\symdiff.src\dependency\test\build\v1\example.c"} {:sourceline 44} true;
+    assert {:sourcefile "c$$users\t-nisebb\documents\symdiff.src\dependency\test\build\regression\test0\test0.c"} {:sourceline 44} true;
     result.TestEmptyRecursion$1 := result.TestEmptyRecursion$2;
     assume value_is(__ctobpl_const_11, result.TestEmptyRecursion$2);
     goto label_1#2;
 
   label_1#2:
-    assert {:sourcefile "c:\users\t-nisebb\documents\symdiff.src\dependency\test\build\v1\example.c"} {:sourceline 45} true;
+    assert {:sourcefile "c$$users\t-nisebb\documents\symdiff.src\dependency\test\build\regression\test0\test0.c"} {:sourceline 45} true;
     return;
 }
 
 
 
-procedure {:extern} TestGlobalRecursion(x_.1: int) returns (result.TestGlobalRecursion$1: int);
+procedure {:extern} TestGlobalRecursion(x.__1: int) returns (result.TestGlobalRecursion$1: int);
   free requires INT_LT(0, alloc);
-  modifies alloc, detChoiceCnt, Res_KERNEL_SOURCE, Res_PROBED, Mem_T.CHAR, Mem_T.FLOAT, Mem_T.INT4;
+  modifies alloc, detChoiceCnt, Mem_T.CHAR, Mem_T.FLOAT, Mem_T.INT4, global1, global2, global3, global4, global5;
   free ensures INT_LEQ(old(alloc), alloc);
-  ensures Subset(Empty(), Empty()) && (forall _r: int :: { Res_KERNEL_SOURCE[_r] } old(Res_KERNEL_SOURCE)[_r] == Res_KERNEL_SOURCE[_r]);
-  free ensures old(Res_KERNEL_SOURCE) == Res_KERNEL_SOURCE;
-  ensures Subset(Empty(), Empty()) && (forall _r: int :: { Res_PROBED[_r] } old(Res_PROBED)[_r] == Res_PROBED[_r]);
-  free ensures old(Res_PROBED) == Res_PROBED;
   free ensures Mem_T.CHAR == old(Mem_T.CHAR);
   free ensures Mem_T.FLOAT == old(Mem_T.FLOAT);
   free ensures Mem_T.INT4 == old(Mem_T.INT4);
 
 
 
-implementation {:extern} TestGlobalRecursion(x_.1: int) returns (result.TestGlobalRecursion$1: int)
+implementation {:extern} TestGlobalRecursion(x.__1: int) returns (result.TestGlobalRecursion$1: int)
 {
   var {:extern} havoc_stringTemp: int;
   var {:extern} condVal: int;
@@ -1089,7 +1013,6 @@ implementation {:extern} TestGlobalRecursion(x_.1: int) returns (result.TestGlob
   var {:extern} tempBoogie17: int;
   var {:extern} tempBoogie18: int;
   var {:extern} tempBoogie19: int;
-  var {:extern} __havoc_dummy_return: int;
 
   anon0#2:
     havoc_stringTemp := 0;
@@ -1099,52 +1022,48 @@ implementation {:extern} TestGlobalRecursion(x_.1: int) returns (result.TestGlob
     result.TestGlobalRecursion$1 := 0;
     result.TestGlobalRecursion$2 := 0;
     x := 0;
-    x := x_.1;
+    x := x.__1;
     goto label_3#2;
 
   label_3#2:
-    assert {:sourcefile "c:\users\t-nisebb\documents\symdiff.src\dependency\test\build\v1\example.c"} {:sourceline 51} true;
-    tempBoogie0 := INT_PLUS(Mem_T.INT4[global2], 1, x);
-    Mem_T.INT4 := Mem_T.INT4[global2 := tempBoogie0];
-    assume value_is(__ctobpl_const_12, Mem_T.INT4[global2]);
+    assert {:sourcefile "c$$users\t-nisebb\documents\symdiff.src\dependency\test\build\regression\test0\test0.c"} {:sourceline 51} true;
+    tempBoogie0 := PLUS(global2, 1, x);
+    global2 := tempBoogie0;
+    assume value_is(__ctobpl_const_12, global2);
     assume value_is(__ctobpl_const_13, x);
     goto label_4#2;
 
   label_4#2:
-    assert {:sourcefile "c:\users\t-nisebb\documents\symdiff.src\dependency\test\build\v1\example.c"} {:sourceline 52} true;
+    assert {:sourcefile "c$$users\t-nisebb\documents\symdiff.src\dependency\test\build\regression\test0\test0.c"} {:sourceline 52} true;
     call result.TestGlobalRecursion$2 := TestGlobalRecursion(x);
     assume value_is(__ctobpl_const_14, x);
     assume value_is(__ctobpl_const_15, x);
     goto label_7#2;
 
   label_7#2:
-    assert {:sourcefile "c:\users\t-nisebb\documents\symdiff.src\dependency\test\build\v1\example.c"} {:sourceline 52} true;
+    assert {:sourcefile "c$$users\t-nisebb\documents\symdiff.src\dependency\test\build\regression\test0\test0.c"} {:sourceline 52} true;
     result.TestGlobalRecursion$1 := result.TestGlobalRecursion$2;
     assume value_is(__ctobpl_const_16, result.TestGlobalRecursion$2);
     goto label_1#2;
 
   label_1#2:
-    assert {:sourcefile "c:\users\t-nisebb\documents\symdiff.src\dependency\test\build\v1\example.c"} {:sourceline 53} true;
+    assert {:sourcefile "c$$users\t-nisebb\documents\symdiff.src\dependency\test\build\regression\test0\test0.c"} {:sourceline 53} true;
     return;
 }
 
 
 
-procedure {:extern} TestRecursion(x_.1: int) returns (result.TestRecursion$1: int);
+procedure {:extern} TestRecursion(x.__1: int) returns (result.TestRecursion$1: int);
   free requires INT_LT(0, alloc);
-  modifies alloc, detChoiceCnt, Res_KERNEL_SOURCE, Res_PROBED, Mem_T.CHAR, Mem_T.FLOAT, Mem_T.INT4;
+  modifies alloc, detChoiceCnt, Mem_T.CHAR, Mem_T.FLOAT, Mem_T.INT4, global1, global2, global3, global4, global5;
   free ensures INT_LEQ(old(alloc), alloc);
-  ensures Subset(Empty(), Empty()) && (forall _r: int :: { Res_KERNEL_SOURCE[_r] } old(Res_KERNEL_SOURCE)[_r] == Res_KERNEL_SOURCE[_r]);
-  free ensures old(Res_KERNEL_SOURCE) == Res_KERNEL_SOURCE;
-  ensures Subset(Empty(), Empty()) && (forall _r: int :: { Res_PROBED[_r] } old(Res_PROBED)[_r] == Res_PROBED[_r]);
-  free ensures old(Res_PROBED) == Res_PROBED;
   free ensures Mem_T.CHAR == old(Mem_T.CHAR);
   free ensures Mem_T.FLOAT == old(Mem_T.FLOAT);
   free ensures Mem_T.INT4 == old(Mem_T.INT4);
 
 
 
-implementation {:extern} TestRecursion(x_.1: int) returns (result.TestRecursion$1: int)
+implementation {:extern} TestRecursion(x.__1: int) returns (result.TestRecursion$1: int)
 {
   var {:extern} havoc_stringTemp: int;
   var {:extern} condVal: int;
@@ -1170,7 +1089,6 @@ implementation {:extern} TestRecursion(x_.1: int) returns (result.TestRecursion$
   var {:extern} tempBoogie17: int;
   var {:extern} tempBoogie18: int;
   var {:extern} tempBoogie19: int;
-  var {:extern} __havoc_dummy_return: int;
 
   anon0#2:
     havoc_stringTemp := 0;
@@ -1180,11 +1098,11 @@ implementation {:extern} TestRecursion(x_.1: int) returns (result.TestRecursion$
     result.TestRecursion$1 := 0;
     result.TestRecursion$2 := 0;
     x := 0;
-    x := x_.1;
+    x := x.__1;
     goto label_3#2;
 
   label_3#2:
-    assert {:sourcefile "c:\users\t-nisebb\documents\symdiff.src\dependency\test\build\v1\example.c"} {:sourceline 57} true;
+    assert {:sourcefile "c$$users\t-nisebb\documents\symdiff.src\dependency\test\build\regression\test0\test0.c"} {:sourceline 57} true;
     goto label_3_true#2, label_3_false#2;
 
   label_3_false#2:
@@ -1193,14 +1111,14 @@ implementation {:extern} TestRecursion(x_.1: int) returns (result.TestRecursion$
     goto label_4#2;
 
   label_4#2:
-    assert {:sourcefile "c:\users\t-nisebb\documents\symdiff.src\dependency\test\build\v1\example.c"} {:sourceline 59} true;
+    assert {:sourcefile "c$$users\t-nisebb\documents\symdiff.src\dependency\test\build\regression\test0\test0.c"} {:sourceline 59} true;
     call result.TestRecursion$2 := TestRecursion(x);
     assume value_is(__ctobpl_const_18, x);
     assume value_is(__ctobpl_const_19, x);
     goto label_8#2;
 
   label_8#2:
-    assert {:sourcefile "c:\users\t-nisebb\documents\symdiff.src\dependency\test\build\v1\example.c"} {:sourceline 59} true;
+    assert {:sourcefile "c$$users\t-nisebb\documents\symdiff.src\dependency\test\build\regression\test0\test0.c"} {:sourceline 59} true;
     result.TestRecursion$1 := result.TestRecursion$2;
     assume value_is(__ctobpl_const_20, result.TestRecursion$2);
     goto label_1#2;
@@ -1211,32 +1129,28 @@ implementation {:extern} TestRecursion(x_.1: int) returns (result.TestRecursion$
     goto label_7#2;
 
   label_7#2:
-    assert {:sourcefile "c:\users\t-nisebb\documents\symdiff.src\dependency\test\build\v1\example.c"} {:sourceline 58} true;
+    assert {:sourcefile "c$$users\t-nisebb\documents\symdiff.src\dependency\test\build\regression\test0\test0.c"} {:sourceline 58} true;
     result.TestRecursion$1 := 0;
     goto label_1#2;
 
   label_1#2:
-    assert {:sourcefile "c:\users\t-nisebb\documents\symdiff.src\dependency\test\build\v1\example.c"} {:sourceline 60} true;
+    assert {:sourcefile "c$$users\t-nisebb\documents\symdiff.src\dependency\test\build\regression\test0\test0.c"} {:sourceline 60} true;
     return;
 }
 
 
 
-procedure {:extern} TestReturnDomination(x_.1: int, w_.1: int) returns (result.TestReturnDomination$1: int);
+procedure {:extern} TestReturnDomination(x.__1: int, w.__1: int) returns (result.TestReturnDomination$1: int);
   free requires INT_LT(0, alloc);
-  modifies alloc, detChoiceCnt, Res_KERNEL_SOURCE, Res_PROBED, Mem_T.CHAR, Mem_T.FLOAT, Mem_T.INT4;
+  modifies alloc, detChoiceCnt, Mem_T.CHAR, Mem_T.FLOAT, Mem_T.INT4, global1, global2, global3, global4, global5;
   free ensures INT_LEQ(old(alloc), alloc);
-  ensures Subset(Empty(), Empty()) && (forall _r: int :: { Res_KERNEL_SOURCE[_r] } old(Res_KERNEL_SOURCE)[_r] == Res_KERNEL_SOURCE[_r]);
-  free ensures old(Res_KERNEL_SOURCE) == Res_KERNEL_SOURCE;
-  ensures Subset(Empty(), Empty()) && (forall _r: int :: { Res_PROBED[_r] } old(Res_PROBED)[_r] == Res_PROBED[_r]);
-  free ensures old(Res_PROBED) == Res_PROBED;
   free ensures Mem_T.CHAR == old(Mem_T.CHAR);
   free ensures Mem_T.FLOAT == old(Mem_T.FLOAT);
   free ensures Mem_T.INT4 == old(Mem_T.INT4);
 
 
 
-implementation {:extern} TestReturnDomination(x_.1: int, w_.1: int) returns (result.TestReturnDomination$1: int)
+implementation {:extern} TestReturnDomination(x.__1: int, w.__1: int) returns (result.TestReturnDomination$1: int)
 {
   var {:extern} havoc_stringTemp: int;
   var {:extern} condVal: int;
@@ -1265,7 +1179,6 @@ implementation {:extern} TestReturnDomination(x_.1: int, w_.1: int) returns (res
   var {:extern} tempBoogie17: int;
   var {:extern} tempBoogie18: int;
   var {:extern} tempBoogie19: int;
-  var {:extern} __havoc_dummy_return: int;
 
   anon0#2:
     havoc_stringTemp := 0;
@@ -1278,37 +1191,36 @@ implementation {:extern} TestReturnDomination(x_.1: int, w_.1: int) returns (res
     x := 0;
     y := 0;
     z := 0;
-    x := x_.1;
-    w := w_.1;
+    x := x.__1;
+    w := w.__1;
     goto label_3#2;
 
   label_3#2:
-    assert {:sourcefile "c:\users\t-nisebb\documents\symdiff.src\dependency\test\build\v1\example.c"} {:sourceline 70} true;
+    assert {:sourcefile "c$$users\t-nisebb\documents\symdiff.src\dependency\test\build\regression\test0\test0.c"} {:sourceline 70} true;
     goto label_4#2;
 
   label_4#2:
-    assert {:sourcefile "c:\users\t-nisebb\documents\symdiff.src\dependency\test\build\v1\example.c"} {:sourceline 70} true;
+    assert {:sourcefile "c$$users\t-nisebb\documents\symdiff.src\dependency\test\build\regression\test0\test0.c"} {:sourceline 70} true;
     goto label_5#2;
 
   label_5#2:
-    assert {:sourcefile "c:\users\t-nisebb\documents\symdiff.src\dependency\test\build\v1\example.c"} {:sourceline 70} true;
+    assert {:sourcefile "c$$users\t-nisebb\documents\symdiff.src\dependency\test\build\regression\test0\test0.c"} {:sourceline 70} true;
     goto label_6#2;
 
   label_6#2:
-    assert {:sourcefile "c:\users\t-nisebb\documents\symdiff.src\dependency\test\build\v1\example.c"} {:sourceline 71} true;
+    assert {:sourcefile "c$$users\t-nisebb\documents\symdiff.src\dependency\test\build\regression\test0\test0.c"} {:sourceline 71} true;
     assume value_is(__ctobpl_const_21, z);
-    z := INT_PLUS(z, 1, 1);
+    z := PLUS(z, 1, 1);
     goto label_7#2;
 
   label_7#2:
-    assert {:sourcefile "c:\users\t-nisebb\documents\symdiff.src\dependency\test\build\v1\example.c"} {:sourceline 72} true;
-    assume value_is(__ctobpl_const_22, Mem_T.INT4[global4]);
-    tempBoogie0 := INT_PLUS(Mem_T.INT4[global4], 1, 1);
-    Mem_T.INT4 := Mem_T.INT4[global4 := tempBoogie0];
+    assert {:sourcefile "c$$users\t-nisebb\documents\symdiff.src\dependency\test\build\regression\test0\test0.c"} {:sourceline 72} true;
+    assume value_is(__ctobpl_const_22, global4);
+    global4 := PLUS(global4, 1, 1);
     goto label_8#2;
 
   label_8#2:
-    assert {:sourcefile "c:\users\t-nisebb\documents\symdiff.src\dependency\test\build\v1\example.c"} {:sourceline 73} true;
+    assert {:sourcefile "c$$users\t-nisebb\documents\symdiff.src\dependency\test\build\regression\test0\test0.c"} {:sourceline 73} true;
     goto label_8_true#2, label_8_false#2;
 
   label_8_false#2:
@@ -1317,10 +1229,9 @@ implementation {:extern} TestReturnDomination(x_.1: int, w_.1: int) returns (res
     goto label_9#2;
 
   label_9#2:
-    assert {:sourcefile "c:\users\t-nisebb\documents\symdiff.src\dependency\test\build\v1\example.c"} {:sourceline 78} true;
-    assume value_is(__ctobpl_const_24, Mem_T.CHAR[global5]);
-    tempBoogie0 := INT_PLUS(Mem_T.CHAR[global5], 1, 1);
-    Mem_T.CHAR := Mem_T.CHAR[global5 := tempBoogie0];
+    assert {:sourcefile "c$$users\t-nisebb\documents\symdiff.src\dependency\test\build\regression\test0\test0.c"} {:sourceline 78} true;
+    assume value_is(__ctobpl_const_24, global5);
+    global5 := PLUS(global5, 1, 1);
     goto label_11#2;
 
   label_8_true#2:
@@ -1329,7 +1240,7 @@ implementation {:extern} TestReturnDomination(x_.1: int, w_.1: int) returns (res
     goto label_10#2;
 
   label_10#2:
-    assert {:sourcefile "c:\users\t-nisebb\documents\symdiff.src\dependency\test\build\v1\example.c"} {:sourceline 74} true;
+    assert {:sourcefile "c$$users\t-nisebb\documents\symdiff.src\dependency\test\build\regression\test0\test0.c"} {:sourceline 74} true;
     goto label_10_true#2, label_10_false#2;
 
   label_10_false#2:
@@ -1338,19 +1249,19 @@ implementation {:extern} TestReturnDomination(x_.1: int, w_.1: int) returns (res
     goto label_11#2;
 
   label_11#2:
-    assert {:sourcefile "c:\users\t-nisebb\documents\symdiff.src\dependency\test\build\v1\example.c"} {:sourceline 79} true;
+    assert {:sourcefile "c$$users\t-nisebb\documents\symdiff.src\dependency\test\build\regression\test0\test0.c"} {:sourceline 79} true;
     assume value_is(__ctobpl_const_26, y);
-    y := INT_PLUS(y, 1, 1);
+    y := PLUS(y, 1, 1);
     goto label_13#2;
 
   label_13#2:
-    assert {:sourcefile "c:\users\t-nisebb\documents\symdiff.src\dependency\test\build\v1\example.c"} {:sourceline 80} true;
-    Mem_T.FLOAT := Mem_T.FLOAT[global3 := 0];
-    assume value_is(__ctobpl_const_27, Mem_T.FLOAT[global3]);
+    assert {:sourcefile "c$$users\t-nisebb\documents\symdiff.src\dependency\test\build\regression\test0\test0.c"} {:sourceline 80} true;
+    global3 := 0;
+    assume value_is(__ctobpl_const_27, global3);
     goto label_14#2;
 
   label_14#2:
-    assert {:sourcefile "c:\users\t-nisebb\documents\symdiff.src\dependency\test\build\v1\example.c"} {:sourceline 81} true;
+    assert {:sourcefile "c$$users\t-nisebb\documents\symdiff.src\dependency\test\build\regression\test0\test0.c"} {:sourceline 81} true;
     result.TestReturnDomination$1 := 2;
     goto label_1#2;
 
@@ -1360,32 +1271,28 @@ implementation {:extern} TestReturnDomination(x_.1: int, w_.1: int) returns (res
     goto label_12#2;
 
   label_12#2:
-    assert {:sourcefile "c:\users\t-nisebb\documents\symdiff.src\dependency\test\build\v1\example.c"} {:sourceline 75} true;
+    assert {:sourcefile "c$$users\t-nisebb\documents\symdiff.src\dependency\test\build\regression\test0\test0.c"} {:sourceline 75} true;
     result.TestReturnDomination$1 := 0;
     goto label_1#2;
 
   label_1#2:
-    assert {:sourcefile "c:\users\t-nisebb\documents\symdiff.src\dependency\test\build\v1\example.c"} {:sourceline 82} true;
+    assert {:sourcefile "c$$users\t-nisebb\documents\symdiff.src\dependency\test\build\regression\test0\test0.c"} {:sourceline 82} true;
     return;
 }
 
 
 
-procedure {:extern} TestSimpleDominationDependancy(y_.1: int, z_.1: int) returns (result.TestSimpleDominationDependancy$1: int);
+procedure {:extern} TestSimpleDominationDependancy(y.__1: int, z.__1: int) returns (result.TestSimpleDominationDependancy$1: int);
   free requires INT_LT(0, alloc);
-  modifies alloc, detChoiceCnt, Res_KERNEL_SOURCE, Res_PROBED, Mem_T.CHAR, Mem_T.FLOAT, Mem_T.INT4;
+  modifies alloc, detChoiceCnt, Mem_T.CHAR, Mem_T.FLOAT, Mem_T.INT4, global1, global2, global3, global4, global5;
   free ensures INT_LEQ(old(alloc), alloc);
-  ensures Subset(Empty(), Empty()) && (forall _r: int :: { Res_KERNEL_SOURCE[_r] } old(Res_KERNEL_SOURCE)[_r] == Res_KERNEL_SOURCE[_r]);
-  free ensures old(Res_KERNEL_SOURCE) == Res_KERNEL_SOURCE;
-  ensures Subset(Empty(), Empty()) && (forall _r: int :: { Res_PROBED[_r] } old(Res_PROBED)[_r] == Res_PROBED[_r]);
-  free ensures old(Res_PROBED) == Res_PROBED;
   free ensures Mem_T.CHAR == old(Mem_T.CHAR);
   free ensures Mem_T.FLOAT == old(Mem_T.FLOAT);
   free ensures Mem_T.INT4 == old(Mem_T.INT4);
 
 
 
-implementation {:extern} TestSimpleDominationDependancy(y_.1: int, z_.1: int) returns (result.TestSimpleDominationDependancy$1: int)
+implementation {:extern} TestSimpleDominationDependancy(y.__1: int, z.__1: int) returns (result.TestSimpleDominationDependancy$1: int)
 {
   var {:extern} havoc_stringTemp: int;
   var {:extern} condVal: int;
@@ -1413,7 +1320,6 @@ implementation {:extern} TestSimpleDominationDependancy(y_.1: int, z_.1: int) re
   var {:extern} tempBoogie17: int;
   var {:extern} tempBoogie18: int;
   var {:extern} tempBoogie19: int;
-  var {:extern} __havoc_dummy_return: int;
 
   anon0#2:
     havoc_stringTemp := 0;
@@ -1425,27 +1331,27 @@ implementation {:extern} TestSimpleDominationDependancy(y_.1: int, z_.1: int) re
     x := 0;
     y := 0;
     z := 0;
-    y := y_.1;
-    z := z_.1;
+    y := y.__1;
+    z := z.__1;
     goto label_3#2;
 
   label_3#2:
-    assert {:sourcefile "c:\users\t-nisebb\documents\symdiff.src\dependency\test\build\v1\example.c"} {:sourceline 34} true;
+    assert {:sourcefile "c$$users\t-nisebb\documents\symdiff.src\dependency\test\build\regression\test0\test0.c"} {:sourceline 34} true;
     goto label_4#2;
 
   label_4#2:
-    assert {:sourcefile "c:\users\t-nisebb\documents\symdiff.src\dependency\test\build\v1\example.c"} {:sourceline 34} true;
-    x := INT_PLUS(y, 1, 1);
+    assert {:sourcefile "c$$users\t-nisebb\documents\symdiff.src\dependency\test\build\regression\test0\test0.c"} {:sourceline 34} true;
+    x := PLUS(y, 1, 1);
     assume value_is(__ctobpl_const_28, x);
     assume value_is(__ctobpl_const_29, y);
     goto label_5#2;
 
   label_5#2:
-    assert {:sourcefile "c:\users\t-nisebb\documents\symdiff.src\dependency\test\build\v1\example.c"} {:sourceline 34} true;
+    assert {:sourcefile "c$$users\t-nisebb\documents\symdiff.src\dependency\test\build\regression\test0\test0.c"} {:sourceline 34} true;
     goto label_6#2;
 
   label_6#2:
-    assert {:sourcefile "c:\users\t-nisebb\documents\symdiff.src\dependency\test\build\v1\example.c"} {:sourceline 35} true;
+    assert {:sourcefile "c$$users\t-nisebb\documents\symdiff.src\dependency\test\build\regression\test0\test0.c"} {:sourceline 35} true;
     goto label_6_true#2, label_6_false#2;
 
   label_6_false#2:
@@ -1459,46 +1365,42 @@ implementation {:extern} TestSimpleDominationDependancy(y_.1: int, z_.1: int) re
     goto label_8#2;
 
   label_8#2:
-    assert {:sourcefile "c:\users\t-nisebb\documents\symdiff.src\dependency\test\build\v1\example.c"} {:sourceline 36} true;
+    assert {:sourcefile "c$$users\t-nisebb\documents\symdiff.src\dependency\test\build\regression\test0\test0.c"} {:sourceline 36} true;
     x := z;
-    assume value_is(__ctobpl_const_32, x);
-    assume value_is(__ctobpl_const_33, z);
+    assume value_is(__ctobpl_const_31, x);
+    assume value_is(__ctobpl_const_32, z);
     goto label_9#2;
 
   label_9#2:
-    assert {:sourcefile "c:\users\t-nisebb\documents\symdiff.src\dependency\test\build\v1\example.c"} {:sourceline 37} true;
+    assert {:sourcefile "c$$users\t-nisebb\documents\symdiff.src\dependency\test\build\regression\test0\test0.c"} {:sourceline 37} true;
     w := 2;
-    assume value_is(__ctobpl_const_34, w);
+    assume value_is(__ctobpl_const_33, w);
     goto label_7#2;
 
   label_7#2:
-    assert {:sourcefile "c:\users\t-nisebb\documents\symdiff.src\dependency\test\build\v1\example.c"} {:sourceline 39} true;
+    assert {:sourcefile "c$$users\t-nisebb\documents\symdiff.src\dependency\test\build\regression\test0\test0.c"} {:sourceline 39} true;
     result.TestSimpleDominationDependancy$1 := w;
-    assume value_is(__ctobpl_const_31, w);
+    assume value_is(__ctobpl_const_34, w);
     goto label_1#2;
 
   label_1#2:
-    assert {:sourcefile "c:\users\t-nisebb\documents\symdiff.src\dependency\test\build\v1\example.c"} {:sourceline 40} true;
+    assert {:sourcefile "c$$users\t-nisebb\documents\symdiff.src\dependency\test\build\regression\test0\test0.c"} {:sourceline 40} true;
     return;
 }
 
 
 
-procedure {:extern} TestSimpleExit(x_.1: int) returns (result.TestSimpleExit$1: int);
+procedure {:extern} TestSimpleExit(x.__1: int) returns (result.TestSimpleExit$1: int);
   free requires INT_LT(0, alloc);
-  modifies alloc, detChoiceCnt, Res_KERNEL_SOURCE, Res_PROBED, Mem_T.CHAR, Mem_T.FLOAT, Mem_T.INT4;
+  modifies alloc, detChoiceCnt, Mem_T.CHAR, Mem_T.FLOAT, Mem_T.INT4, global1, global2, global3, global4, global5;
   free ensures INT_LEQ(old(alloc), alloc);
-  ensures Subset(Empty(), Empty()) && (forall _r: int :: { Res_KERNEL_SOURCE[_r] } old(Res_KERNEL_SOURCE)[_r] == Res_KERNEL_SOURCE[_r]);
-  free ensures old(Res_KERNEL_SOURCE) == Res_KERNEL_SOURCE;
-  ensures Subset(Empty(), Empty()) && (forall _r: int :: { Res_PROBED[_r] } old(Res_PROBED)[_r] == Res_PROBED[_r]);
-  free ensures old(Res_PROBED) == Res_PROBED;
   free ensures Mem_T.CHAR == old(Mem_T.CHAR);
   free ensures Mem_T.FLOAT == old(Mem_T.FLOAT);
   free ensures Mem_T.INT4 == old(Mem_T.INT4);
 
 
 
-implementation {:extern} TestSimpleExit(x_.1: int) returns (result.TestSimpleExit$1: int)
+implementation {:extern} TestSimpleExit(x.__1: int) returns (result.TestSimpleExit$1: int)
 {
   var {:extern} havoc_stringTemp: int;
   var {:extern} condVal: int;
@@ -1524,7 +1426,6 @@ implementation {:extern} TestSimpleExit(x_.1: int) returns (result.TestSimpleExi
   var {:extern} tempBoogie17: int;
   var {:extern} tempBoogie18: int;
   var {:extern} tempBoogie19: int;
-  var {:extern} __havoc_dummy_return: int;
 
   anon0#2:
     havoc_stringTemp := 0;
@@ -1534,11 +1435,11 @@ implementation {:extern} TestSimpleExit(x_.1: int) returns (result.TestSimpleExi
     result.TestSimpleExit$1 := 0;
     result.exit$2 := 0;
     x := 0;
-    x := x_.1;
+    x := x.__1;
     goto label_3#2;
 
   label_3#2:
-    assert {:sourcefile "c:\users\t-nisebb\documents\symdiff.src\dependency\test\build\v1\example.c"} {:sourceline 86} true;
+    assert {:sourcefile "c$$users\t-nisebb\documents\symdiff.src\dependency\test\build\regression\test0\test0.c"} {:sourceline 86} true;
     call result.exit$2 := det_choice();
     assume false;
     return;
